src/program_proof/tulip/program/gcoord/group_preparer.v
@@ -1,0 +1,1553 @@
+From Perennial.program_proof.tulip.invariance Require Import propose.
+From Perennial.program_proof.tulip.program Require Import prelude.
+From Perennial.program_proof.tulip.program Require Import quorum count_bool_map.
+
+Local Ltac Zify.zify_post_hook ::= Z.div_mod_to_equations.
+
+Inductive gppphase :=
+| GPPValidating
+| GPPPreparing
+| GPPUnpreparing
+| GPPWaiting
+| GPPPrepared
+| GPPCommitted
+| GPPAborted.
+
+Definition gppphase_to_u64 phase :=
+  match phase with
+  | GPPValidating => (W64 0)
+  | GPPPreparing => (W64 1)
+  | GPPUnpreparing => (W64 2)
+  | GPPWaiting => (W64 3)
+  | GPPPrepared => (W64 4)
+  | GPPCommitted => (W64 5)
+  | GPPAborted => (W64 6)
+  end.
+
+#[global]
+Instance gppphase_to_u64_inj :
+  Inj eq eq gppphase_to_u64.
+Proof. intros x y H. by destruct x, y. Defined.
+
+Inductive gppaction :=
+| GPPFastPrepare
+| GPPValidate
+| GPPPrepare
+| GPPUnprepare
+| GPPQuery
+| GPPRefresh.
+
+Definition gppaction_to_u64 action :=
+  match action with
+  | GPPFastPrepare => (W64 0)
+  | GPPValidate => (W64 1)
+  | GPPPrepare => (W64 2)
+  | GPPUnprepare => (W64 3)
+  | GPPQuery => (W64 4)
+  | GPPRefresh => (W64 5)
+  end.
+
+#[global]
+Instance gppaction_to_u64_inj :
+  Inj eq eq gppaction_to_u64.
+Proof. intros x y H. by destruct x, y. Defined.
+
+Definition gpp_ready phase :=
+  match phase with
+  | GPPValidating => False
+  | GPPPreparing => False
+  | GPPUnpreparing => False
+  | GPPWaiting => False
+  | GPPPrepared => True
+  | GPPCommitted => True
+  | GPPAborted => True
+  end.
+
+#[global]
+Instance gpp_ready_decision phase :
+  Decision (gpp_ready phase).
+Proof. destruct phase; apply _. Defined.
+
+Section repr.
+  Context `{!heapGS Σ, !tulip_ghostG Σ}.
+
+  (*@ type GroupPreparer struct {                                             @*)
+  (*@     // Number of replicas. Read-only.                                   @*)
+  (*@     nrps   uint64                                                       @*)
+  (*@     // Control phase.                                                   @*)
+  (*@     phase  uint64                                                       @*)
+  (*@     // Fast-path replica responses.                                     @*)
+  (*@     frespm map[uint64]bool                                              @*)
+  (*@     // Replicas validated.                                              @*)
+  (*@     vdm    map[uint64]bool                                              @*)
+  (*@     // Slow-path replica responses.                                     @*)
+  (*@     // NB: The range doesn't need to be bool, unit would suffice.       @*)
+  (*@     srespm map[uint64]bool                                              @*)
+  (*@     //                                                                  @*)
+  (*@     // TODO: Merge @validated and @sresps                               @*)
+  (*@     // @phase = VALIDATING => records whether a certain replica is validated; @*)
+  (*@     // @phase = PREPARING / UNPREPARING => records prepared/unprepared. @*)
+  (*@     //                                                                  @*)
+  (*@ }                                                                       @*)
+  Definition own_group_preparer_nrps (gpp : loc) : iProp Σ :=
+    ∃ (nrps : u64),
+      "Hnrps"   ∷ gpp ↦[GroupPreparer :: "nrps"] #nrps ∗
+      "%Hnrps"  ∷ ⌜uint.nat nrps = size rids_all⌝.
+
+  Definition own_group_preparer_phase (gpp : loc) (phase : gppphase) : iProp Σ :=
+    ∃ (phaseW : u64),
+      "HphaseP" ∷ gpp ↦[GroupPreparer :: "phase"] #phaseW ∗
+      "%Hphase" ∷ ⌜gppphase_to_u64 phase = phaseW⌝.
+
+  Definition fast_prepare_responses γ ts gid (frespm : gmap u64 bool) : iProp Σ :=
+    [∗ map] rid ↦ p ∈ frespm,
+      is_replica_pdec_at_rank γ gid rid ts O p ∗
+      (if p then is_replica_validated_ts γ gid rid ts else True).
+
+  Definition validation_responses γ ts gid (vdm : gmap u64 bool) : iProp Σ :=
+    ([∗ set] rid ∈ dom vdm, is_replica_validated_ts γ gid rid ts).
+
+  Definition slow_prepare_responses γ ts gid phase (srespm : gmap u64 bool) : iProp Σ :=
+    match phase with
+    | GPPValidating => True
+    | GPPPreparing =>
+        ([∗ set] rid ∈ dom srespm, is_replica_pdec_at_rank γ gid rid ts 1%nat true)
+    | GPPUnpreparing =>
+        ([∗ set] rid ∈ dom srespm, is_replica_pdec_at_rank γ gid rid ts 1%nat false)
+    | GPPWaiting => True
+    | GPPPrepared => True
+    | GPPCommitted => True
+    | GPPAborted => True
+    end.
+
+  #[global]
+  Instance slow_prepare_responses_persistent γ ts gid phase srespm :
+    Persistent (slow_prepare_responses γ ts gid phase srespm).
+  Proof. destruct phase; apply _. Defined.
+
+  Definition safe_group_preparer_phase γ ts gid phase : iProp Σ :=
+    match phase with
+    | GPPValidating => True
+    | GPPPreparing =>
+        quorum_validated γ gid ts ∗ is_group_prepare_proposal γ gid ts 1%nat true
+    | GPPUnpreparing => is_group_prepare_proposal γ gid ts 1%nat false
+    | GPPWaiting => True
+    | GPPPrepared =>
+        quorum_prepared γ gid ts ∗ quorum_validated γ gid ts
+    | GPPCommitted => ∃ wrs, is_txn_committed γ ts wrs
+    | GPPAborted => is_txn_aborted γ ts ∨ quorum_unprepared γ gid ts
+    end.
+
+  #[global]
+  Instance safe_group_preparer_phase_persistent γ ts gid phase :
+    Persistent (safe_group_preparer_phase γ ts gid phase).
+  Proof. destruct phase; apply _. Defined.
+
+  Definition slow_path_permission γ ts gid phase : iProp Σ :=
+    match phase with
+    | GPPValidating => own_txn_client_token γ ts gid
+    | GPPPreparing => True
+    | GPPUnpreparing => True
+    | GPPWaiting => True
+    | GPPPrepared => True
+    | GPPCommitted => True
+    | GPPAborted => True
+    end.
+
+  Definition own_group_preparer_frespm (gpp : loc) ts gid γ : iProp Σ :=
+    ∃ (frespmP : loc) (frespm : gmap u64 bool),
+      "HfrespmP" ∷ gpp ↦[GroupPreparer :: "frespm"] #frespmP ∗
+      "Hfrespm"  ∷ own_map frespmP (DfracOwn 1) frespm ∗
+      "#Hfast"   ∷ fast_prepare_responses γ ts gid frespm ∗
+      "%Hfincl"  ∷ ⌜dom frespm ⊆ rids_all⌝.
+
+  Definition own_group_preparer_vdm (gpp : loc) ts gid γ : iProp Σ :=
+    ∃ (vdmP : loc) (vdm : gmap u64 bool),
+      "HvdmP"        ∷ gpp ↦[GroupPreparer :: "vdm"] #vdmP ∗
+      "Hvdm"         ∷ own_map vdmP (DfracOwn 1) vdm ∗
+      "#Hvalidation" ∷ validation_responses γ ts gid vdm ∗
+      "%Hvincl"      ∷ ⌜dom vdm ⊆ rids_all⌝.
+
+  Definition own_srespm_map_conditional
+    phase srespmP (srespm : gmap u64 bool) : iProp Σ :=
+    match phase with
+    | GPPValidating => True
+    | GPPPreparing => own_map srespmP (DfracOwn 1) srespm
+    | GPPUnpreparing => own_map srespmP (DfracOwn 1) srespm
+    | GPPWaiting => True
+    | GPPPrepared => True
+    | GPPCommitted => True
+    | GPPAborted => True
+    end.
+
+  Definition own_group_preparer_srespm (gpp : loc) (phase : gppphase) ts gid γ : iProp Σ :=
+    ∃ (srespmP : loc) (srespm : gmap u64 bool),
+      "HsrespmP" ∷ gpp ↦[GroupPreparer :: "srespm"] #srespmP ∗
+      "Hsrespm"  ∷ own_srespm_map_conditional phase srespmP srespm ∗
+      "#Hslow"   ∷ slow_prepare_responses γ ts gid phase srespm ∗
+      "%Hsincl"  ∷ ⌜dom srespm ⊆ rids_all⌝.
+
+  Definition own_group_preparer_with_phase
+    (gpp : loc) (phase : gppphase) ts gid γ : iProp Σ :=
+      "Hnrps"   ∷ own_group_preparer_nrps gpp ∗
+      "Hphase"  ∷ own_group_preparer_phase gpp phase ∗
+      "Hfrespm" ∷ own_group_preparer_frespm gpp ts gid γ ∗
+      "Hvdm"    ∷ own_group_preparer_vdm gpp ts gid γ ∗
+      "Hsrespm" ∷ own_group_preparer_srespm gpp phase ts gid γ ∗
+      "Htxncli" ∷ slow_path_permission γ ts gid phase ∗
+      "#Hsafe"  ∷ safe_group_preparer_phase γ ts gid phase.
+
+  Definition own_group_preparer (gpp : loc) ts gid γ : iProp Σ :=
+    ∃ (phase : gppphase),
+      "Hgpp" ∷ own_group_preparer_with_phase gpp phase ts gid γ.
+
+End repr.
+
+Section program.
+  Context `{!heapGS Σ, !tulip_ghostG Σ}.
+
+  Theorem wp_GroupPreparer__cquorum (gpp : loc) (n : u64) :
+    {{{ own_group_preparer_nrps gpp }}}
+      GroupPreparer__cquorum #gpp #n
+    {{{ RET #(bool_decide (size rids_all / 2 < uint.Z n)); own_group_preparer_nrps gpp }}}.
+  Proof.
+    iIntros (Φ) "Hgpp HΦ".
+    wp_rec.
+
+    (*@ func (gpp *GroupPreparer) cquorum(n uint64) bool {                      @*)
+    (*@     return quorum.ClassicQuorum(gpp.nrps) <= n                          @*)
+    (*@ }                                                                       @*)
+    iNamed "Hgpp".
+    wp_loadField.
+    wp_apply wp_ClassicQuorum.
+    iIntros (x Hx).
+    wp_pures.
+    case_bool_decide as Hc1.
+    { case_bool_decide as Hc2; last word.
+      iApply "HΦ". by iFrame "∗ %".
+    }
+    { case_bool_decide as Hc2; first word.
+      iApply "HΦ". by iFrame "∗ %".
+    }
+  Qed.
+
+  Theorem wp_GroupPreparer__fquorum (gpp : loc) (n : u64) :
+    {{{ own_group_preparer_nrps gpp }}}
+      GroupPreparer__fquorum #gpp #n
+    {{{ RET #(bool_decide (((3 * size rids_all + 3) / 4 ≤ uint.Z n) ∧ size rids_all ≠ O));
+        own_group_preparer_nrps gpp
+    }}}.
+  Proof.
+    iIntros (Φ) "Hgpp HΦ".
+    wp_rec.
+
+    (*@ func (gpp *GroupPreparer) fquorum(n uint64) bool {                      @*)
+    (*@     return quorum.FastQuorum(gpp.nrps) <= n                             @*)
+    (*@ }                                                                       @*)
+    iNamed "Hgpp".
+    wp_loadField.
+    wp_apply wp_FastQuorum.
+    { rewrite size_rids_all in Hnrps. word. }
+    iIntros (x Hx).
+    wp_pures.
+    case_bool_decide as Hc1.
+    { case_bool_decide as Hc2; last word.
+      iApply "HΦ". by iFrame "∗ %".
+    }
+    { case_bool_decide as Hc2.
+      { exfalso.
+        apply Classical_Prop.not_and_or in Hc1.
+        destruct Hc1 as [Hc1 | Hz]; last first.
+        { rewrite size_rids_all in Hz. lia. }
+        word.
+      }
+      iApply "HΦ". by iFrame "∗ %".
+    }
+  Qed.
+
+  Theorem wp_GroupPreparer__hcquorum (gpp : loc) (n : u64) :
+    {{{ own_group_preparer_nrps gpp }}}
+      GroupPreparer__hcquorum #gpp #n
+    {{{ RET #(bool_decide (size rids_all / 4 + 1 ≤ uint.Z n));
+        own_group_preparer_nrps gpp
+    }}}.
+  Proof.
+    iIntros (Φ) "Hgpp HΦ".
+    wp_rec.
+
+    (*@ func (gpp *GroupPreparer) hcquorum(n uint64) bool {                     @*)
+    (*@     return quorum.Half(quorum.ClassicQuorum(gpp.nrps)) <= n             @*)
+    (*@ }                                                                       @*)
+    iNamed "Hgpp".
+    wp_loadField.
+    wp_apply wp_ClassicQuorum.
+    iIntros (x Hx).
+    wp_apply wp_Half.
+    { clear -Hx. word. }
+    iIntros (y Hy).
+    wp_pures.
+    case_bool_decide as Hc1.
+    { case_bool_decide as Hc2; last first.
+      { exfalso. clear -Hnrps Hx Hy Hc1 Hc2. word. }
+      iApply "HΦ". by iFrame "∗ %".
+    }
+    { case_bool_decide as Hc2.
+      { exfalso. clear -Hnrps Hx Hy Hc1 Hc2. word. }
+      iApply "HΦ". by iFrame "∗ %".
+    }
+  Qed.
+
+  Theorem wp_GroupPreparer__ready (gpp : loc) phase :
+    {{{ own_group_preparer_phase gpp phase }}}
+      GroupPreparer__ready #gpp
+    {{{ RET #(bool_decide (gpp_ready phase)); own_group_preparer_phase gpp phase }}}.
+  Proof.
+    iIntros (Φ) "Hgpp HΦ".
+    wp_rec.
+
+    (*@ func (gpp *GroupPreparer) ready() bool {                                @*)
+    (*@     return GPP_PREPARED <= gpp.phase                                    @*)
+    (*@ }                                                                       @*)
+    iNamed "Hgpp".
+    wp_loadField.
+    wp_pures.
+    rewrite /gppphase_to_u64 in Hphase.
+    rewrite /gpp_ready.
+    case_bool_decide as Hcond.
+    { case_bool_decide as Hret.
+      { iApply "HΦ". by iFrame. }
+      destruct phase; word.
+    }
+    { case_bool_decide as Hret; last first.
+      { iApply "HΦ". by iFrame. }
+      destruct phase; word.
+    }
+  Qed.
+
+  Definition try_resign_requirement γ ts (res : rpres) : iProp Σ :=
+    match res with
+    | ReplicaOK => True
+    | ReplicaCommittedTxn => (∃ wrs, is_txn_committed γ ts wrs)
+    | ReplicaAbortedTxn => is_txn_aborted γ ts
+    | ReplicaStaleCoordinator => True
+    | ReplicaFailedValidation => True
+    | ReplicaInvalidRank => True
+    | ReplicaWrongLeader => True
+    end.
+
+  #[global]
+  Instance try_resign_requirement_persistent γ ts res :
+    Persistent (try_resign_requirement γ ts res).
+  Proof. destruct res; apply _. Defined.
+
+  Definition not_finalizing_rpres (res : rpres) :=
+    match res with
+    | ReplicaOK => True
+    | ReplicaCommittedTxn => False
+    | ReplicaAbortedTxn => False
+    | ReplicaStaleCoordinator => False
+    | ReplicaFailedValidation => True
+    | ReplicaInvalidRank => True
+    | ReplicaWrongLeader => True
+    end.
+
+  Theorem wp_GroupPreparer__tryResign (gpp : loc) (res : rpres) ts gid γ :
+    try_resign_requirement γ ts res -∗
+    {{{ own_group_preparer gpp ts gid γ }}}
+      GroupPreparer__tryResign #gpp #(rpres_to_u64 res)
+    {{{ (resigned : bool), RET #resigned; 
+        own_group_preparer gpp ts gid γ ∗
+        ⌜if resigned then True else not_finalizing_rpres res⌝
+    }}}.
+  Proof.
+    iIntros "#Hreq" (Φ) "!> Hgpp HΦ".
+    wp_rec.
+
+    (*@ func (gpp *GroupPreparer) tryResign(res uint64) bool {                  @*)
+    (*@     if gpp.ready() {                                                    @*)
+    (*@         return true                                                     @*)
+    (*@     }                                                                   @*)
+    (*@                                                                         @*)
+    do 2 iNamed "Hgpp".
+    wp_apply (wp_GroupPreparer__ready with "Hphase").
+    iIntros "Hphase".
+    case_bool_decide as Hready; wp_pures.
+    { iApply "HΦ". by iFrame. }
+
+    (*@     if res == tulip.REPLICA_COMMITTED_TXN {                             @*)
+    (*@         gpp.phase = GPP_COMMITTED                                       @*)
+    (*@         return true                                                     @*)
+    (*@     }                                                                   @*)
+    (*@                                                                         @*)
+    case_bool_decide as Hcmted; wp_pures.
+    { iNamed "Hphase".
+      destruct res; try done.
+      wp_storeField.
+      iApply "HΦ".
+      iModIntro.
+      iSplit; last done.
+      iExists GPPCommitted.
+      iFrame "∗ # %".
+      iSplit; first done.
+      iNamed "Hsrespm".
+      by iFrame "∗ %".
+    }
+
+    (*@     if res == tulip.REPLICA_ABORTED_TXN {                               @*)
+    (*@         gpp.phase = GPP_ABORTED                                         @*)
+    (*@         return true                                                     @*)
+    (*@     }                                                                   @*)
+    (*@                                                                         @*)
+    case_bool_decide as Habted; wp_pures.
+    { iNamed "Hphase".
+      destruct res; try done.
+      wp_storeField.
+      iApply "HΦ".
+      iModIntro.
+      iSplit; last done.
+      iExists GPPAborted.
+      iFrame "∗ # %".
+      iSplit; first done.
+      iNamed "Hsrespm".
+      by iFrame "∗ %".
+    }
+
+    (*@     if res == tulip.REPLICA_STALE_COORDINATOR {                         @*)
+    (*@         return true                                                     @*)
+    (*@     }                                                                   @*)
+    (*@                                                                         @*)
+    case_bool_decide as Hstale; wp_pures.
+    { iApply "HΦ". by iFrame. }
+
+    (*@     return false                                                        @*)
+    (*@ }                                                                       @*)
+    iApply "HΦ".
+    iFrame "∗ # %".
+    iPureIntro.
+    by destruct res.
+  Qed.
+
+  Theorem wp_GroupPreparer__tryFastAbort (gpp : loc) ts gid γ :
+    {{{ own_group_preparer gpp ts gid γ }}}
+      GroupPreparer__tryFastAbort #gpp
+    {{{ (aborted : bool), RET #aborted; own_group_preparer gpp ts gid γ }}}.
+  Proof.
+    iIntros (Φ) "Hgpp HΦ".
+    wp_rec.
+
+    (*@ func (gpp *GroupPreparer) tryFastAbort() bool {                         @*)
+    (*@     // Count how many replicas have fast unprepared.                    @*)
+    (*@     n := util.CountBoolMap(gpp.frespm, false)                           @*)
+    (*@                                                                         @*)
+    do 2 iNamed "Hgpp". iNamed "Hfrespm".
+    wp_loadField.
+    wp_apply (wp_CountBoolMap with "Hfrespm").
+    iIntros (n) "[Hfrespm %Hn]".
+    iAssert (own_group_preparer_frespm gpp ts gid γ)%I
+      with "[HfrespmP Hfrespm]" as "Hfrespm".
+    { by iFrame "∗ # %". }
+
+    (*@     // Move to the ABORTED phase if obtaining a fast quorum of fast unprepares. @*)
+    (*@     if gpp.fquorum(n) {                                                 @*)
+    (*@         gpp.phase = GPP_ABORTED                                         @*)
+    (*@         return true                                                     @*)
+    (*@     }                                                                   @*)
+    (*@     return false                                                        @*)
+    (*@ }                                                                       @*)
+    wp_apply (wp_GroupPreparer__fquorum with "Hnrps").
+    iIntros "Hnrps".
+    case_bool_decide as Hfq; wp_pures.
+    { iNamed "Hphase".
+      wp_storeField.
+      iApply "HΦ".
+      iModIntro.
+      iExists GPPAborted.
+      iFrame "∗ #".
+      iSplit; first done.
+      iSplitL "Hsrespm".
+      { iNamed "Hsrespm". by iFrame "∗ %". }
+      iSplit; first done.
+      iRight.
+      iExists O.
+      rewrite /quorum_pdec_at_rank.
+      case_decide; last done.
+      set frespmq := filter _ _ in Hn.
+      iExists (dom frespmq).
+      iSplit; last first.
+      { iPureIntro.
+        split.
+        { etrans; last apply Hfincl. apply dom_filter_subseteq. }
+        { destruct Hfq as [Hfq Hnz].
+          split; last done.
+          rewrite size_dom.
+          clear -Hfq Hn. word.
+        }
+      }
+      rewrite /fast_prepare_responses.
+      iDestruct (big_sepM_subseteq _ _ frespmq with "Hfast") as "Hfastq".
+      { apply map_filter_subseteq. }
+      rewrite big_sepS_big_sepM.
+      iApply (big_sepM_mono with "Hfastq").
+      iIntros (rid b Hb) "[Hpdec _]".
+      apply map_lookup_filter_Some in Hb as [_ Hb]. simpl in Hb.
+      by subst b.
+    }
+    iApply "HΦ".
+    by iFrame "∗ # %".
+  Qed.
+
+  Theorem wp_GroupPreparer__tryFastPrepare (gpp : loc) ts gid γ :
+    {{{ own_group_preparer gpp ts gid γ }}}
+      GroupPreparer__tryFastPrepare #gpp
+    {{{ (prepared : bool), RET #prepared; own_group_preparer gpp ts gid γ }}}.
+  Proof.
+    iIntros (Φ) "Hgpp HΦ".
+    wp_rec.
+
+    (*@ func (gpp *GroupPreparer) tryFastPrepare() bool {                       @*)
+    (*@     // Count how many replicas have fast prepared.                      @*)
+    (*@     n := util.CountBoolMap(gpp.frespm, true)                            @*)
+    (*@                                                                         @*)
+    do 2 iNamed "Hgpp". iNamed "Hfrespm".
+    wp_loadField.
+    wp_apply (wp_CountBoolMap with "Hfrespm").
+    iIntros (n) "[Hfrespm %Hn]".
+    iAssert (own_group_preparer_frespm gpp ts gid γ)%I
+      with "[HfrespmP Hfrespm]" as "Hfrespm".
+    { by iFrame "∗ # %". }
+
+    (*@     // Move to the PREPARED phase if obtaining a fast quorum of fast prepares. @*)
+    (*@     if gpp.fquorum(n) {                                                 @*)
+    (*@         gpp.phase = GPP_PREPARED                                        @*)
+    (*@         return true                                                     @*)
+    (*@     }                                                                   @*)
+    (*@     return false                                                        @*)
+    (*@ }                                                                       @*)
+    wp_apply (wp_GroupPreparer__fquorum with "Hnrps").
+    iIntros "Hnrps".
+    case_bool_decide as Hfq; wp_pures.
+    { iNamed "Hphase".
+      wp_storeField.
+      iApply "HΦ".
+      iModIntro.
+      iExists GPPPrepared.
+      iFrame "∗ #".
+      iSplit; first done.
+      iSplitL "Hsrespm".
+      { iNamed "Hsrespm". by iFrame "∗ %". }
+      iSplit; first done.
+      set frespmq := filter _ _ in Hn.
+      iSplit.
+      { (* Prove [quorum_prepared]. *)
+        iExists O.
+        rewrite /quorum_pdec_at_rank.
+        case_decide; last done.
+        iExists (dom frespmq).
+        iSplit; last first.
+        { iPureIntro.
+          split.
+          { etrans; last apply Hfincl. apply dom_filter_subseteq. }
+          { destruct Hfq as [Hfq Hnz].
+            split; last done.
+            rewrite size_dom.
+            clear -Hfq Hn. word.
+          }
+        }
+        rewrite /fast_prepare_responses.
+        iDestruct (big_sepM_subseteq _ _ frespmq with "Hfast") as "Hfastq".
+        { apply map_filter_subseteq. }
+        rewrite big_sepS_big_sepM.
+        iApply (big_sepM_mono with "Hfastq").
+        iIntros (rid b Hb) "[Hpdec _]".
+        apply map_lookup_filter_Some in Hb as [_ Hb]. simpl in Hb.
+        by subst b.
+      }
+      { (* Prove [quorum_validated]. *)
+        iExists (dom frespmq).
+        iSplit; last first.
+        { iPureIntro.
+          split.
+          { etrans; last apply Hfincl. apply dom_filter_subseteq. }
+          { destruct Hfq as [Hfq Hnz].
+            rewrite /cquorum_size size_dom.
+            clear -Hfq Hn Hnz. word.
+          }
+        }
+        rewrite /fast_prepare_responses.
+        iDestruct (big_sepM_subseteq _ _ frespmq with "Hfast") as "Hfastq".
+        { apply map_filter_subseteq. }
+        iDestruct (big_sepM_sep with "Hfastq") as "[_ Hvdq]".
+        rewrite big_sepS_big_sepM.
+        iApply (big_sepM_mono with "Hvdq").
+        iIntros (rid b Hb) "Hvd".
+        apply map_lookup_filter_Some in Hb as [_ Hb]. simpl in Hb.
+        by subst b.
+      }
+    }
+    iApply "HΦ".
+    by iFrame "∗ # %".
+  Qed.
+
+  Theorem wp_GroupPreparer__tryBecomePreparing (gpp : loc) ts gid γ :
+    gid ∈ gids_all ->
+    know_tulip_inv γ -∗
+    {{{ own_group_preparer_with_phase gpp GPPValidating ts gid γ }}}
+      GroupPreparer__tryBecomePreparing #gpp
+    {{{ RET #(); own_group_preparer gpp ts gid γ }}}.
+  Proof.
+    iIntros (Hgid) "#Hinv".
+    iIntros (Φ) "!> Hgpp HΦ".
+    wp_rec.
+
+    (*@ func (gpp *GroupPreparer) tryBecomePreparing() {                        @*)
+    (*@     // Count how many replicas have validated.                          @*)
+    (*@     nvd := uint64(len(gpp.vdm))                                         @*)
+    (*@     if !gpp.cquorum(nvd) {                                              @*)
+    (*@         // Cannot move to the PREPARING phase unless some classic quorum of @*)
+    (*@         // replicas successfully validate.                              @*)
+    (*@         return                                                          @*)
+    (*@     }                                                                   @*)
+    (*@                                                                         @*)
+    iNamed "Hgpp". iNamed "Hvdm".
+    wp_loadField.
+    wp_apply (wp_MapLen with "Hvdm").
+    iIntros "[%Hnvdmnoof Hvdm]".
+    iAssert (own_group_preparer_vdm gpp ts gid γ)%I with "[HvdmP Hvdm]" as "Hvdm".
+    { iFrame "∗ # %". }
+    wp_apply (wp_GroupPreparer__cquorum with "Hnrps").
+    iIntros "Hnrps".
+    case_bool_decide as Hnvd; wp_pures; last first.
+    { iApply "HΦ". by iFrame "∗ #". }
+
+    (*@     // Count how many replicas have responded in the fast path.         @*)
+    (*@     nresp := uint64(len(gpp.frespm))                                    @*)
+    (*@     if !gpp.cquorum(nresp) {                                            @*)
+    (*@         return                                                          @*)
+    (*@     }                                                                   @*)
+    (*@                                                                         @*)
+    iNamed "Hfrespm".
+    wp_loadField.
+    wp_apply (wp_MapLen with "Hfrespm").
+    iIntros "[%Hnrespmnoof Hfrespm]".
+    wp_apply (wp_GroupPreparer__cquorum with "Hnrps").
+    iIntros "Hnrps".
+    case_bool_decide as Hnresp; wp_pures; last first.
+    { iApply "HΦ". by iFrame "∗ # %". }
+
+    (*@     // Count how many replicas have prepared.                           @*)
+    (*@     nfp := util.CountBoolMap(gpp.frespm, true)                          @*)
+    (*@     if !gpp.hcquorum(nfp) {                                             @*)
+    (*@         // Cannot move to the PREPARING phase unless half (i.e., celing(n / 2)) @*)
+    (*@         // of replicas in some classic quorum agrees to prepare.        @*)
+    (*@         return                                                          @*)
+    (*@     }                                                                   @*)
+    (*@                                                                         @*)
+    wp_loadField.
+    wp_apply (wp_CountBoolMap with "Hfrespm").
+    iIntros (nfp) "[Hfrespm %Hnfp]".
+    wp_apply (wp_GroupPreparer__hcquorum with "Hnrps").
+    iIntros "Hnrps".
+    case_bool_decide as Hhcq; wp_pures; last first.
+    { iApply "HΦ". by iFrame "∗ # %". }
+    (* Prove [safe_proposal γ gid ts 1%nat true] to propose [true] at rank 1 for [ts]. *)
+    iAssert (safe_proposal γ gid ts 1%nat true)%I as "#Hsafepsl".
+    { simpl.
+      iDestruct (big_sepM_sep with "Hfast") as "[Hpdecx _]".
+      rewrite /is_replica_pdec_at_rank.
+      iDestruct (big_sepM_exists_sepM2 with "Hpdecx") as (bm) "Hpdecy".
+      iDestruct (big_sepM2_and with "Hpdecy") as "[Hpdec Hacpt]".
+      iDestruct (big_sepM2_pure with "Hacpt") as %[_ Hacpt].
+      iDestruct (big_sepM2_dom with "Hpdec") as %Hdombm.
+      assert (Hcq : cquorum rids_all (dom bm)).
+      { rewrite -Hdombm.
+        split; first apply Hfincl.
+        rewrite /cquorum_size size_dom.
+        clear -Hnresp. word.
+      }
+      iExists bm.
+      set sc := size rids_all.
+      simpl.
+      assert (latest_before_quorum 1 bm = O) as ->.
+      { unshelve epose proof (latest_before_quorum_lt bm 1%nat _ _) as Hltone.
+        { rewrite -dom_empty_iff_L. by eapply cquorum_non_empty_q. }
+        { done. }
+        lia.
+      }
+      iSplit.
+      { iApply (big_sepM2_sepM_impl with "Hpdec"); first done.
+        iIntros (rid b l1 l2 Hb Hl1 Hl2) "!> #Hlb".
+        rewrite Hl1 in Hl2. by inv Hl2.
+      }
+      iSplit; first done.
+      iPureIntro.
+      split; first apply Hcq.
+      split.
+      { intros k l Hl.
+        assert (is_Some (frespm !! k)) as [b Hb].
+        { by rewrite -elem_of_dom Hdombm elem_of_dom. }
+        specialize (Hacpt _ _ _ Hb Hl).
+        apply lookup_lt_Some in Hacpt.
+        clear -Hacpt. lia.
+      }
+      simpl.
+      assert (Heq : (uint.nat nfp ≤ nfast bm true)%nat).
+      { rewrite Hnfp /nfast -2!size_dom.
+        apply subseteq_size.
+        intros x Hx.
+        apply elem_of_dom in Hx as [b Hb].
+        apply map_lookup_filter_Some in Hb as [Hb Heq].
+        simpl in Heq. subst b.
+        assert (is_Some (bm !! x)) as [l Hl].
+        { by rewrite -elem_of_dom -Hdombm elem_of_dom. }
+        specialize (Hacpt _ _ _ Hb Hl).
+        apply elem_of_dom.
+        exists l.
+        by apply map_lookup_filter_Some.
+      }
+      clear -Hhcq Heq. word.
+    }
+
+    (*@     gpp.srespm = make(map[uint64]bool)                                  @*)
+    (*@     gpp.phase = GPP_PREPARING                                           @*)
+    (*@                                                                         @*)
+    iNamed "Hsrespm".
+    wp_apply wp_NewMap.
+    iClear "Hsrespm".
+    iIntros (srespmP') "Hsrespm".
+    wp_storeField.
+    iNamed "Hphase".
+    simpl.
+    wp_storeField.
+    iAssert (own_group_preparer_frespm gpp ts gid γ)%I
+      with "[HfrespmP Hfrespm]" as "Hfrespm".
+    { iFrame "∗ # %". }
+    iAssert (own_group_preparer_phase gpp GPPPreparing)%I
+      with "[HphaseP]" as "Hphase".
+    { by iFrame. }
+    iAssert (own_group_preparer_srespm gpp GPPPreparing ts gid γ)%I
+      with "[HsrespmP Hsrespm]" as "Hsrespm".
+    { iFrame. by rewrite /= dom_empty_L big_sepS_empty. }
+
+    (*@     // Logical action: Propose.                                         @*)
+    (*@ }                                                                       @*)
+    iInv "Hinv" as "> HinvO" "HinvC".
+    iNamed "HinvO".
+    simpl.
+    iDestruct (big_sepS_elem_of_acc with "Hgroups") as "[Hgroup HgroupsC]".
+    { apply Hgid. }
+    iMod (group_inv_propose with "Hsafepsl [Htxncli] Hgroup") as "[Hgroup #Hppsl]".
+    { done. }
+    { by rewrite /exclusive_proposal /=. }
+    iDestruct ("HgroupsC" with "Hgroup") as "Hgroups".
+    iMod ("HinvC" with "[$Htxnsys $Hkeys $Hgroups $Hrgs]") as "_".
+    iApply "HΦ".
+    iFrame "∗ #".
+    iPureIntro.
+    split; first apply Hvincl.
+    rewrite /cquorum_size size_dom.
+    clear -Hnvd. word.
+  Qed.
+
+  Theorem wp_GroupPreparer__tryBecomeUnpreparing (gpp : loc) ts gid γ :
+    gid ∈ gids_all ->
+    know_tulip_inv γ -∗
+    {{{ own_group_preparer_with_phase gpp GPPValidating ts gid γ }}}
+      GroupPreparer__tryBecomeUnpreparing #gpp
+    {{{ RET #(); own_group_preparer gpp ts gid γ }}}.
+  Proof.
+    iIntros (Hgid) "#Hinv".
+    iIntros (Φ) "!> Hgpp HΦ".
+    wp_rec.
+
+    (*@ func (gpp *GroupPreparer) tryBecomeUnpreparing() {                      @*)
+    (*@     // Count how many replicas have responded in the fast path.         @*)
+    (*@     nresp := uint64(len(gpp.frespm))                                    @*)
+    (*@     if !gpp.cquorum(nresp) {                                            @*)
+    (*@         return                                                          @*)
+    (*@     }                                                                   @*)
+    (*@                                                                         @*)
+    iNamed "Hgpp".
+    iNamed "Hfrespm".
+    wp_loadField.
+    wp_apply (wp_MapLen with "Hfrespm").
+    iIntros "[%Hnrespmnoof Hfrespm]".
+    wp_apply (wp_GroupPreparer__cquorum with "Hnrps").
+    iIntros "Hnrps".
+    case_bool_decide as Hnresp; wp_pures; last first.
+    { iApply "HΦ". by iFrame "∗ # %". }
+
+    (*@     // Count how many replicas have unprepared.                         @*)
+    (*@     nfu := util.CountBoolMap(gpp.frespm, false)                         @*)
+    (*@     if !gpp.hcquorum(nfu) {                                             @*)
+    (*@         // Cannot move to the UNPREPARING phase unless half of replicas in some @*)
+    (*@         // classic quorum agrees to unprepare.                          @*)
+    (*@         return                                                          @*)
+    (*@     }                                                                   @*)
+    (*@                                                                         @*)
+    wp_loadField.
+    wp_apply (wp_CountBoolMap with "Hfrespm").
+    iIntros (nfp) "[Hfrespm %Hnfp]".
+    wp_apply (wp_GroupPreparer__hcquorum with "Hnrps").
+    iIntros "Hnrps".
+    case_bool_decide as Hhcq; wp_pures; last first.
+    { iApply "HΦ". by iFrame "∗ # %". }
+    (* Prove [safe_proposal γ gid ts 1%nat true] to propose [true] at rank 1 for [ts]. *)
+    iAssert (safe_proposal γ gid ts 1%nat false)%I as "#Hsafepsl".
+    { simpl.
+      iDestruct (big_sepM_sep with "Hfast") as "[Hpdecx _]".
+      rewrite /is_replica_pdec_at_rank.
+      iDestruct (big_sepM_exists_sepM2 with "Hpdecx") as (bm) "Hpdecy".
+      iDestruct (big_sepM2_and with "Hpdecy") as "[Hpdec Hacpt]".
+      iDestruct (big_sepM2_pure with "Hacpt") as %[_ Hacpt].
+      iDestruct (big_sepM2_dom with "Hpdec") as %Hdombm.
+      assert (Hcq : cquorum rids_all (dom bm)).
+      { rewrite -Hdombm.
+        split; first apply Hfincl.
+        rewrite /cquorum_size size_dom.
+        clear -Hnresp. word.
+      }
+      iExists bm.
+      set sc := size rids_all.
+      simpl.
+      assert (latest_before_quorum 1 bm = O) as ->.
+      { unshelve epose proof (latest_before_quorum_lt bm 1%nat _ _) as Hltone.
+        { rewrite -dom_empty_iff_L. by eapply cquorum_non_empty_q. }
+        { done. }
+        lia.
+      }
+      iSplit.
+      { iApply (big_sepM2_sepM_impl with "Hpdec"); first done.
+        iIntros (rid b l1 l2 Hb Hl1 Hl2) "!> #Hlb".
+        rewrite Hl1 in Hl2. by inv Hl2.
+      }
+      iSplit; first done.
+      iPureIntro.
+      split; first apply Hcq.
+      split.
+      { intros k l Hl.
+        assert (is_Some (frespm !! k)) as [b Hb].
+        { by rewrite -elem_of_dom Hdombm elem_of_dom. }
+        specialize (Hacpt _ _ _ Hb Hl).
+        apply lookup_lt_Some in Hacpt.
+        clear -Hacpt. lia.
+      }
+      simpl.
+      assert (Heq : (uint.nat nfp ≤ nfast bm false)%nat).
+      { rewrite Hnfp /nfast -2!size_dom.
+        apply subseteq_size.
+        intros x Hx.
+        apply elem_of_dom in Hx as [b Hb].
+        apply map_lookup_filter_Some in Hb as [Hb Heq].
+        simpl in Heq. subst b.
+        assert (is_Some (bm !! x)) as [l Hl].
+        { by rewrite -elem_of_dom -Hdombm elem_of_dom. }
+        specialize (Hacpt _ _ _ Hb Hl).
+        apply elem_of_dom.
+        exists l.
+        by apply map_lookup_filter_Some.
+      }
+      clear -Hhcq Heq. word.
+    }
+
+    (*@     gpp.srespm = make(map[uint64]bool)                                  @*)
+    (*@     gpp.phase = GPP_UNPREPARING                                         @*)
+    (*@                                                                         @*)
+    iNamed "Hsrespm".
+    wp_apply wp_NewMap.
+    iClear "Hsrespm".
+    iIntros (srespmP') "Hsrespm".
+    wp_storeField.
+    iNamed "Hphase".
+    simpl.
+    wp_storeField.
+    iAssert (own_group_preparer_frespm gpp ts gid γ)%I
+      with "[HfrespmP Hfrespm]" as "Hfrespm".
+    { iFrame "∗ # %". }
+    iAssert (own_group_preparer_phase gpp GPPUnpreparing)%I
+      with "[HphaseP]" as "Hphase".
+    { by iFrame. }
+    iAssert (own_group_preparer_srespm gpp GPPUnpreparing ts gid γ)%I
+      with "[HsrespmP Hsrespm]" as "Hsrespm".
+    { iFrame. by rewrite /= dom_empty_L big_sepS_empty. }
+
+    (*@     // Logical action: Propose.                                         @*)
+    (*@ }                                                                       @*)
+    iInv "Hinv" as "> HinvO" "HinvC".
+    iNamed "HinvO".
+    simpl.
+    iDestruct (big_sepS_elem_of_acc with "Hgroups") as "[Hgroup HgroupsC]".
+    { apply Hgid. }
+    iMod (group_inv_propose with "Hsafepsl [Htxncli] Hgroup") as "[Hgroup #Hppsl]".
+    { done. }
+    { by rewrite /exclusive_proposal /=. }
+    iDestruct ("HgroupsC" with "Hgroup") as "Hgroups".
+    iMod ("HinvC" with "[$Htxnsys $Hkeys $Hgroups $Hrgs]") as "_".
+    iApply "HΦ".
+    by iFrame "∗ #".
+  Qed.
+
+  Theorem wp_GroupPreparer__collectFastDecision
+    (gpp : loc) (rid : u64) (b : bool) ts gid γ :
+    rid ∈ rids_all ->
+    is_replica_pdec_at_rank γ gid rid ts O b -∗
+    (if b then is_replica_validated_ts γ gid rid ts else True) -∗
+    {{{ own_group_preparer gpp ts gid γ }}}
+      GroupPreparer__collectFastDecision #gpp #rid #b
+    {{{ RET #(); own_group_preparer gpp ts gid γ }}}.
+  Proof.
+    iIntros (Hrid) "#Hpdec #Hvd".
+    iIntros (Φ) "!> Hgpp HΦ".
+    wp_rec.
+
+    (*@ func (gpp *GroupPreparer) collectFastDecision(rid uint64, b bool) {     @*)
+    (*@     gpp.frespm[rid] = b                                                 @*)
+    (*@ }                                                                       @*)
+    do 2 iNamed "Hgpp". iNamed "Hfrespm".
+    wp_loadField.
+    wp_apply (wp_MapInsert with "Hfrespm"); first done.
+    iIntros "Hfrespm".
+    wp_pures.
+    iApply "HΦ".
+    iFrame "∗ # %".
+    iModIntro.
+    iSplit.
+    { iApply (big_sepM_insert_2 with "[] Hfast"). iFrame "#". }
+    iPureIntro.
+    rewrite dom_insert_L.
+    set_solver.
+  Qed.
+
+  Theorem wp_GroupPreparer__collectValidation (gpp : loc) (rid : u64) phase ts gid γ :
+    rid ∈ rids_all ->
+    is_replica_validated_ts γ gid rid ts -∗
+    {{{ own_group_preparer_with_phase gpp phase ts gid γ }}}
+      GroupPreparer__collectValidation #gpp #rid
+    {{{ RET #(); own_group_preparer_with_phase gpp phase ts gid γ }}}.
+  Proof.
+    iIntros (Hrid) "#Hvd".
+    iIntros (Φ) "!> Hgpp HΦ".
+    wp_rec.
+
+    (*@ func (gpp *GroupPreparer) collectValidation(rid uint64) {               @*)
+    (*@     gpp.vdm[rid] = true                                                 @*)
+    (*@ }                                                                       @*)
+    iNamed "Hgpp". iNamed "Hvdm".
+    wp_loadField.
+    wp_apply (wp_MapInsert with "Hvdm"); first done.
+    iIntros "Hvdm".
+    wp_pures.
+    iApply "HΦ".
+    iFrame "Hfrespm ∗ # %".
+    iModIntro.
+    iSplit.
+    { rewrite /validation_responses dom_insert_L.
+      by iApply (big_sepS_insert_2 with "[] Hvalidation").
+    }
+    iPureIntro.
+    rewrite dom_insert_L.
+    set_solver.
+  Qed.
+
+  Theorem wp_GroupPreparer__in (gpp : loc) (phase : gppphase) ts gid γ :
+    {{{ own_group_preparer gpp ts gid γ }}}
+      GroupPreparer__in #gpp #(gppphase_to_u64 phase)
+    {{{ (ok : bool), RET #ok; 
+        if ok
+        then own_group_preparer_with_phase gpp phase ts gid γ
+        else own_group_preparer gpp ts gid γ
+    }}}.
+  Proof.
+    iIntros (Φ) "Hgpp HΦ".
+    wp_rec.
+
+    (*@ func (gpp *GroupPreparer) in(phase uint64) bool {                       @*)
+    (*@     return gpp.phase == phase                                           @*)
+    (*@ }                                                                       @*)
+    rename phase into phasearg.
+    do 2 iNamed "Hgpp". iNamed "Hphase".
+    wp_loadField.
+    wp_pures.
+    iApply "HΦ".
+    case_bool_decide as Hok; last first.
+    { by iFrame "∗ # %". }
+    symmetry in Hok. inv Hok.
+    by iFrame "∗ # %".
+  Qed.
+
+  Theorem wp_GroupPreparer__processFastPrepareResult
+    (gpp : loc) (rid : u64) (res : rpres) ts gid γ :
+    gid ∈ gids_all ->
+    rid ∈ rids_all ->
+    fast_prepare_outcome γ gid rid ts res -∗
+    know_tulip_inv γ -∗
+    {{{ own_group_preparer gpp ts gid γ }}}
+      GroupPreparer__processFastPrepareResult #gpp #rid #(rpres_to_u64 res)
+    {{{ RET #(); own_group_preparer gpp ts gid γ }}}.
+  Proof.
+    iIntros (Hgid Hrid) "#Hfp #Hinv".
+    iIntros (Φ) "!> Hgpp HΦ".
+    wp_rec.
+
+    (*@ func (gpp *GroupPreparer) processFastPrepareResult(rid uint64, res uint64) { @*)
+    (*@     // Result is ready or a backup coordinator has become live.         @*)
+    (*@     if gpp.tryResign(res) {                                             @*)
+    (*@         return                                                          @*)
+    (*@     }                                                                   @*)
+    (*@                                                                         @*)
+    wp_apply (wp_GroupPreparer__tryResign with "[] Hgpp").
+    { by destruct res. }
+    iIntros (resigned) "[Hgpp %Hresigned]".
+    destruct resigned; wp_pures.
+    { by iApply "HΦ". }
+
+    (*@     // Fast-prepare fails; fast abort if possible.                      @*)
+    (*@     if res == tulip.REPLICA_FAILED_VALIDATION {                         @*)
+    (*@         gpp.collectFastDecision(rid, false)                             @*)
+    (*@                                                                         @*)
+    case_bool_decide as Hres; wp_pures.
+    { destruct res; try done. simpl.
+      wp_apply (wp_GroupPreparer__collectFastDecision with "Hfp [] Hgpp").
+      { apply Hrid. }
+      { done. }
+      iIntros "Hgpp".
+
+      (*@         aborted := gpp.tryFastAbort()                                   @*)
+      (*@         if aborted {                                                    @*)
+      (*@             return                                                      @*)
+      (*@         }                                                               @*)
+      (*@                                                                         @*)
+      wp_apply (wp_GroupPreparer__tryFastAbort with "Hgpp").
+      iIntros (aborted) "Hgpp".
+      wp_pures.
+      destruct aborted; wp_pures.
+      { by iApply "HΦ". }
+
+      (*@         if !gpp.in(GPP_VALIDATING) {                                    @*)
+      (*@             return                                                      @*)
+      (*@         }                                                               @*)
+      (*@                                                                         @*)
+      wp_apply (wp_GroupPreparer__in _ GPPValidating with "Hgpp").
+      iIntros (validating) "Hgpp".
+      destruct validating; wp_pures; last first.
+      { by iApply "HΦ". }
+
+      (*@         gpp.tryBecomeUnpreparing()                                      @*)
+      (*@         return                                                          @*)
+      (*@     }                                                                   @*)
+      (*@                                                                         @*)
+      wp_apply (wp_GroupPreparer__tryBecomeUnpreparing with "Hinv Hgpp").
+      { apply Hgid. }
+      iIntros "Hgpp".
+      wp_pures.
+      iApply "HΦ".
+      by iFrame.
+    }
+    (* Prove [res = ReplicaOK]. *)
+    destruct res; try done.
+
+    (*@     // Fast-prepare succeeds; fast prepare if possible.                 @*)
+    (*@     gpp.collectFastDecision(rid, true)                                  @*)
+    (*@     if gpp.tryFastPrepare() {                                           @*)
+    (*@         return                                                          @*)
+    (*@     }                                                                   @*)
+    (*@                                                                         @*)
+    iDestruct "Hfp" as "[Hvd Hpdec]".
+    wp_apply (wp_GroupPreparer__collectFastDecision with "Hpdec Hvd Hgpp").
+    { apply Hrid. }
+    iIntros "Hgpp".
+    wp_apply (wp_GroupPreparer__tryFastPrepare with "Hgpp").
+    iIntros (prepared) "Hgpp".
+    destruct prepared; wp_pures.
+    { by iApply "HΦ". }
+
+    (*@     // Ignore the result if it's not in the validating phase. At this point, the @*)
+    (*@     // other possible phases are preparing and unpreparing.             @*)
+    (*@     if !gpp.in(GPP_VALIDATING) {                                        @*)
+    (*@         return                                                          @*)
+    (*@     }                                                                   @*)
+    (*@                                                                         @*)
+    wp_apply (wp_GroupPreparer__in _ GPPValidating with "Hgpp").
+    iIntros (validating) "Hgpp".
+    destruct validating; wp_pures; last first.
+    { by iApply "HΦ". }
+
+    (*@     // Record success of validation and try to move to the preparing phase. @*)
+    (*@     gpp.collectValidation(rid)                                          @*)
+    (*@     gpp.tryBecomePreparing()                                            @*)
+    (*@ }                                                                       @*)
+    wp_apply (wp_GroupPreparer__collectValidation with "Hvd Hgpp").
+    { apply Hrid. }
+    iIntros "Hgpp".
+    wp_apply (wp_GroupPreparer__tryBecomePreparing with "Hinv Hgpp").
+    { apply Hgid. }
+    iIntros "Hgpp".
+    wp_pures.
+    iApply "HΦ".
+    by iFrame.
+  Qed.
+
+  Theorem wp_GroupPreparer__processValidateResult
+    (gpp : loc) (rid : u64) (res : rpres) ts gid γ :
+    gid ∈ gids_all ->
+    rid ∈ rids_all ->
+    validate_outcome γ gid rid ts res -∗
+    know_tulip_inv γ -∗
+    {{{ own_group_preparer gpp ts gid γ }}}
+      GroupPreparer__processValidateResult #gpp #rid #(rpres_to_u64 res)
+    {{{ RET #(); own_group_preparer gpp ts gid γ }}}.
+  Proof.
+    iIntros (Hgid Hrid) "#Hvd #Hinv".
+    iIntros (Φ) "!> Hgpp HΦ".
+    wp_rec.
+
+    (*@ func (gpp *GroupPreparer) processValidateResult(rid uint64, res uint64) { @*)
+    (*@     // Result is ready or a backup coordinator has become live.         @*)
+    (*@     if gpp.tryResign(res) {                                             @*)
+    (*@         return                                                          @*)
+    (*@     }                                                                   @*)
+    (*@                                                                         @*)
+    wp_apply (wp_GroupPreparer__tryResign with "[] Hgpp").
+    { by destruct res. }
+    iIntros (resigned) "[Hgpp %Hresigned]".
+    destruct resigned; wp_pures.
+    { by iApply "HΦ". }
+
+    (*@     // Validation fails; nothing to record.                             @*)
+    (*@     if res == tulip.REPLICA_FAILED_VALIDATION {                         @*)
+    (*@         return                                                          @*)
+    (*@     }                                                                   @*)
+    (*@                                                                         @*)
+    case_bool_decide as Hres; wp_pures.
+    { by iApply "HΦ". }
+    (* Prove [res = ReplicaOK]. *)
+    destruct res; try done.
+
+    (*@     // Skip if the coordiantor is not in the validating phase. At this point, @*)
+    (*@     // the other possible phases are preparing and unpreparing.         @*)
+    (*@     if !gpp.in(GPP_VALIDATING) {                                        @*)
+    (*@         return                                                          @*)
+    (*@     }                                                                   @*)
+    (*@                                                                         @*)
+    wp_apply (wp_GroupPreparer__in _ GPPValidating with "Hgpp").
+    iIntros (validating) "Hgpp".
+    destruct validating; wp_pures; last first.
+    { by iApply "HΦ". }
+
+    (*@     // Record success of validation and try to move to the preparing phase. @*)
+    (*@     gpp.collectValidation(rid)                                          @*)
+    (*@     gpp.tryBecomePreparing()                                            @*)
+    (*@ }                                                                       @*)
+    wp_apply (wp_GroupPreparer__collectValidation with "Hvd Hgpp").
+    { apply Hrid. }
+    iIntros "Hgpp".
+    wp_apply (wp_GroupPreparer__tryBecomePreparing with "Hinv Hgpp").
+    { apply Hgid. }
+    iIntros "Hgpp".
+    wp_pures.
+    iApply "HΦ".
+    by iFrame.
+  Qed.
+
+  Theorem wp_GroupPreparer__processPrepareResult
+    (gpp : loc) (rid : u64) (res : rpres) ts gid γ :
+    rid ∈ rids_all ->
+    accept_outcome γ gid rid ts 1%nat true res -∗
+    {{{ own_group_preparer gpp ts gid γ }}}
+      GroupPreparer__processPrepareResult #gpp #rid #(rpres_to_u64 res)
+    {{{ RET #(); own_group_preparer gpp ts gid γ }}}.
+  Proof.
+    iIntros (Hrid) "#Hvd".
+    iIntros (Φ) "!> Hgpp HΦ".
+    wp_rec.
+
+    (*@ func (gpp *GroupPreparer) processPrepareResult(rid uint64, res uint64) { @*)
+    (*@     // Result is ready or a backup coordinator has become live.         @*)
+    (*@     if gpp.tryResign(res) {                                             @*)
+    (*@         return                                                          @*)
+    (*@     }                                                                   @*)
+    (*@                                                                         @*)
+    wp_apply (wp_GroupPreparer__tryResign with "[] Hgpp").
+    { by destruct res. }
+    iIntros (resigned) "[Hgpp %Hresigned]".
+    destruct resigned; wp_pures.
+    { by iApply "HΦ". }
+    (* Prove [res = ReplicaOK]. *)
+    destruct res; try done. simpl.
+
+    (*@     // We might be able to prove this without an additional check.      @*)
+    (*@     if !gpp.in(GPP_PREPARING) {                                         @*)
+    (*@         return                                                          @*)
+    (*@     }                                                                   @*)
+    (*@                                                                         @*)
+    wp_apply (wp_GroupPreparer__in _ GPPPreparing with "Hgpp").
+    iIntros (preparing) "Hgpp".
+    destruct preparing; wp_pures; last first.
+    { by iApply "HΦ". }
+
+    (*@     // Record success of preparing the replica and try to move to prepared. @*)
+    (*@     gpp.srespm[rid] = true                                              @*)
+    (*@                                                                         @*)
+    iNamed "Hgpp". iNamed "Hsrespm".
+    wp_loadField.
+    wp_apply (wp_MapInsert with "Hsrespm"); first done.
+    iIntros "Hsrespm".
+
+    (*@     // Count how many replicas have prepared.                           @*)
+    (*@     n := uint64(len(gpp.srespm))                                        @*)
+    (*@                                                                         @*)
+    wp_loadField.
+    wp_apply (wp_MapLen with "Hsrespm").
+    iIntros "[%Hn Hsrespm]".
+    wp_pures.
+
+    (*@     // Go to prepared phase if successful prepares reaches a classic quorum. @*)
+    (*@     if gpp.cquorum(n) {                                                 @*)
+    (*@         gpp.phase = GPP_PREPARED                                        @*)
+    (*@     }                                                                   @*)
+    (*@ }                                                                       @*)
+    wp_apply (wp_GroupPreparer__cquorum with "Hnrps").
+    iIntros "Hnrps".
+    case_bool_decide as Hq; wp_pures.
+    { iNamed "Hphase".
+      wp_storeField.
+      iApply "HΦ".
+      iAssert (own_group_preparer_phase gpp GPPPrepared)%I with "[HphaseP]" as "Hphase".
+      { by iFrame. }
+      simpl.
+      iDestruct (big_sepS_insert_2 rid with "[] Hslow") as "Hslow'".
+      { iFrame "Hvd". }
+      iAssert (own_group_preparer_srespm gpp GPPPrepared ts gid γ)%I
+        with "[HsrespmP Hsrespm]" as "Hsrespm".
+      { iFrame. simpl.
+        iExists ∅. (* just a placeholder *)
+        do 2 (iSplit; first done).
+        iPureIntro.
+        (* rewrite dom_insert_L. *)
+        clear -Hrid Hsincl. set_solver.
+      }
+      iModIntro.
+      iFrame "∗ # %".
+      simpl.
+      iDestruct "Hsafe" as "[Hqv _]".
+      iFrame "Hqv".
+      iExists 1%nat.
+      rewrite /quorum_pdec_at_rank /=.
+      set ridsq := _ ∪ _.
+      iExists ridsq.
+      iSplit; first done.
+      iPureIntro.
+      split.
+      { clear-Hsincl Hrid. set_solver. }
+      { rewrite /cquorum_size.
+        destruct (decide (rid ∈ dom srespm)) as [Hin | Hnotin].
+        { assert (ridsq = dom srespm) as -> by set_solver.
+          rewrite size_dom.
+          apply elem_of_dom in Hin.
+          rewrite map_size_insert_Some in Hn Hq; last apply Hin.
+          clear -Hn Hq. word.
+        }
+        subst ridsq.
+        rewrite size_union; last set_solver.
+        rewrite size_singleton size_dom.
+        apply not_elem_of_dom in Hnotin.
+        rewrite map_size_insert_None in Hn Hq; last apply Hnotin.
+        clear -Hn Hq. word.
+      }
+    }
+    iApply "HΦ".
+    iAssert (own_group_preparer_srespm gpp GPPPreparing ts gid γ)%I
+      with "[HsrespmP Hsrespm]" as "Hsrespm".
+    { iFrame. simpl.
+      iSplit.
+      { rewrite dom_insert_L.
+        iApply (big_sepS_insert_2 with "[] Hslow").
+        iFrame "Hvd".
+      }
+      iPureIntro.
+      rewrite dom_insert_L.
+      clear -Hrid Hsincl. set_solver.
+    }
+    by iFrame "∗ # %".
+  Qed.
+
+  Theorem wp_GroupPreparer__processUnprepareResult
+    (gpp : loc) (rid : u64) (res : rpres) ts gid γ :
+    rid ∈ rids_all ->
+    accept_outcome γ gid rid ts 1%nat false res -∗
+    {{{ own_group_preparer gpp ts gid γ }}}
+      GroupPreparer__processUnprepareResult #gpp #rid #(rpres_to_u64 res)
+    {{{ RET #(); own_group_preparer gpp ts gid γ }}}.
+  Proof.
+    iIntros (Hrid) "#Hvd".
+    iIntros (Φ) "!> Hgpp HΦ".
+    wp_rec.
+
+    (*@ func (gpp *GroupPreparer) processUnprepareResult(rid uint64, res uint64) { @*)
+    (*@     // Result is ready or a backup coordinator has become live.         @*)
+    (*@     if gpp.tryResign(res) {                                             @*)
+    (*@         return                                                          @*)
+    (*@     }                                                                   @*)
+    (*@                                                                         @*)
+    wp_apply (wp_GroupPreparer__tryResign with "[] Hgpp").
+    { by destruct res. }
+    iIntros (resigned) "[Hgpp %Hresigned]".
+    destruct resigned; wp_pures.
+    { by iApply "HΦ". }
+    (* Prove [res = ReplicaOK]. *)
+    destruct res; try done. simpl.
+
+    (*@     // We might be able to prove this without an additional check.      @*)
+    (*@     if !gpp.in(GPP_UNPREPARING) {                                       @*)
+    (*@         return                                                          @*)
+    (*@     }                                                                   @*)
+    (*@                                                                         @*)
+    wp_apply (wp_GroupPreparer__in _ GPPUnpreparing with "Hgpp").
+    iIntros (unpreparing) "Hgpp".
+    destruct unpreparing; wp_pures; last first.
+    { by iApply "HΦ". }
+
+    (*@     // Record success of unpreparing the replica and try to move to aborted. @*)
+    (*@     gpp.srespm[rid] = true                                              @*)
+    (*@                                                                         @*)
+    iNamed "Hgpp". iNamed "Hsrespm".
+    wp_loadField.
+    wp_apply (wp_MapInsert with "Hsrespm"); first done.
+    iIntros "Hsrespm".
+
+    (*@     // Count how many replicas have unprepared.                         @*)
+    (*@     n := uint64(len(gpp.srespm))                                        @*)
+    (*@                                                                         @*)
+    wp_loadField.
+    wp_apply (wp_MapLen with "Hsrespm").
+    iIntros "[%Hn Hsrespm]".
+    wp_pures.
+
+    (*@     // Go to aborted phase if successful unprepares reaches a classic quorum. @*)
+    (*@     if gpp.cquorum(n) {                                                 @*)
+    (*@         gpp.phase = GPP_ABORTED                                         @*)
+    (*@     }                                                                   @*)
+    (*@ }                                                                       @*)
+    wp_apply (wp_GroupPreparer__cquorum with "Hnrps").
+    iIntros "Hnrps".
+    case_bool_decide as Hq; wp_pures.
+    { iNamed "Hphase".
+      wp_storeField.
+      iApply "HΦ".
+      iAssert (own_group_preparer_phase gpp GPPAborted)%I with "[HphaseP]" as "Hphase".
+      { by iFrame. }
+      simpl.
+      iDestruct (big_sepS_insert_2 rid with "[] Hslow") as "Hslow'".
+      { iFrame "Hvd". }
+      iAssert (own_group_preparer_srespm gpp GPPAborted ts gid γ)%I
+        with "[HsrespmP Hsrespm]" as "Hsrespm".
+      { iFrame. simpl.
+        iExists ∅. (* just a placeholder *)
+        do 2 (iSplit; first done).
+        iPureIntro.
+        (* rewrite dom_insert_L. *)
+        clear -Hrid Hsincl. set_solver.
+      }
+      iModIntro.
+      iFrame "∗ # %".
+      iRight.
+      iExists 1%nat.
+      rewrite /quorum_pdec_at_rank /=.
+      set ridsq := _ ∪ _.
+      iExists ridsq.
+      iSplit; first done.
+      iPureIntro.
+      split.
+      { clear-Hsincl Hrid. set_solver. }
+      { rewrite /cquorum_size.
+        destruct (decide (rid ∈ dom srespm)) as [Hin | Hnotin].
+        { assert (ridsq = dom srespm) as -> by set_solver.
+          rewrite size_dom.
+          apply elem_of_dom in Hin.
+          rewrite map_size_insert_Some in Hn Hq; last apply Hin.
+          clear -Hn Hq. word.
+        }
+        subst ridsq.
+        rewrite size_union; last set_solver.
+        rewrite size_singleton size_dom.
+        apply not_elem_of_dom in Hnotin.
+        rewrite map_size_insert_None in Hn Hq; last apply Hnotin.
+        clear -Hn Hq. word.
+      }
+    }
+    iApply "HΦ".
+    iAssert (own_group_preparer_srespm gpp GPPUnpreparing ts gid γ)%I
+      with "[HsrespmP Hsrespm]" as "Hsrespm".
+    { iFrame. simpl.
+      iSplit.
+      { rewrite dom_insert_L.
+        iApply (big_sepS_insert_2 with "[] Hslow").
+        iFrame "Hvd".
+      }
+      iPureIntro.
+      rewrite dom_insert_L.
+      clear -Hrid Hsincl. set_solver.
+    }
+    by iFrame "∗ # %".
+  Qed.
+
+  Theorem wp_GroupPreparer__processQueryResult
+    (gpp : loc) (rid : u64) (res : rpres) ts gid γ :
+    rid ∈ rids_all ->
+    query_outcome γ ts res -∗
+    {{{ own_group_preparer gpp ts gid γ }}}
+      GroupPreparer__processQueryResult #gpp #rid #(rpres_to_u64 res)
+    {{{ RET #(); own_group_preparer gpp ts gid γ }}}.
+  Proof.
+    iIntros (Hrid) "#Hquery".
+    iIntros (Φ) "!> Hgpp HΦ".
+    wp_rec.
+
+    (*@ func (gpp *GroupPreparer) processQueryResult(rid uint64, res uint64) {  @*)
+    (*@     // Result is ready or a backup coordinator has become live.         @*)
+    (*@     gpp.tryResign(res)                                                  @*)
+    (*@ }                                                                       @*)
+    wp_apply (wp_GroupPreparer__tryResign with "[] Hgpp").
+    { by destruct res. }
+    iIntros (resigned) "[Hgpp %Hresigned]".
+    wp_pures.
+    by iApply "HΦ".
+  Qed.
+
+  Definition safe_gppaction γ ts gid action : iProp Σ :=
+    match action with
+    | GPPFastPrepare => True
+    | GPPValidate => True
+    | GPPPrepare => is_group_prepare_proposal γ gid ts 1%nat true
+    | GPPUnprepare => is_group_prepare_proposal γ gid ts 1%nat false
+    | GPPQuery => True
+    | GPPRefresh => True
+    end.
+
+  Theorem wp_GroupPreparer__action (gpp : loc) (rid : u64) γ ts gid :
+    {{{ own_group_preparer gpp ts gid γ }}}
+      GroupPreparer__action #gpp #rid
+    {{{ (action : gppaction), RET #(gppaction_to_u64 action); 
+        own_group_preparer gpp ts gid γ ∗
+        safe_gppaction γ ts gid action
+    }}}.
+  Proof.
+    iIntros (Φ) "Hgpp HΦ".
+    wp_rec.
+
+    (*@ func (gpp *GroupPreparer) action(rid uint64) uint64 {                   @*)
+    (*@     // Validate the transaction through fast-path or slow-path.         @*)
+    (*@     if gpp.phase == GPP_VALIDATING {                                    @*)
+    (*@         // Check if the fast-path response for replica @rid is available. @*)
+    (*@         _, fresp := gpp.frespm[rid]                                     @*)
+    (*@         if !fresp {                                                     @*)
+    (*@             // Have not received the fast-path response.                @*)
+    (*@             return GPP_FAST_PREPARE                                     @*)
+    (*@         }                                                               @*)
+    (*@                                                                         @*)
+    wp_pures.
+    wp_apply (wp_GroupPreparer__in _ GPPValidating with "Hgpp").
+    iIntros (validting) "Hgpp".
+    destruct validting; wp_pures.
+    { iNamed "Hgpp".
+      iNamed "Hfrespm".
+      wp_loadField.
+      wp_apply (wp_MapGet with "Hfrespm").
+      iIntros (b1 fresp) "[_ Hfrespm]".
+      wp_pures.
+      destruct fresp; wp_pures; last first.
+      { iApply ("HΦ" $! GPPFastPrepare). by iFrame "∗ # %". }
+
+      (*@         // Check if the validation response for replica @rid is available. @*)
+      (*@         _, validated := gpp.vdm[rid]                                    @*)
+      (*@         if !validated {                                                 @*)
+      (*@             // Previous attemp of validation fails; retry.              @*)
+      (*@             return GPP_VALIDATE                                         @*)
+      (*@         }                                                               @*)
+      (*@                                                                         @*)
+      iNamed "Hvdm".
+      wp_loadField.
+      wp_apply (wp_MapGet with "Hvdm").
+      iIntros (b2 validated) "[_ Hvdm]".
+      wp_pures.
+      destruct validated; wp_pures; last first.
+      { iApply ("HΦ" $! GPPValidate). by iFrame "HfrespmP HvdmP ∗ # %". }
+
+      (*@         // Successfully validated (in either fast-path or slow-path).   @*)
+      (*@         return GPP_QUERY                                                @*)
+      (*@     }                                                                   @*)
+      (*@                                                                         @*)
+      { iApply ("HΦ" $! GPPQuery). by iFrame "HfrespmP HvdmP ∗ # %". }
+    }
+
+    (*@     // Prepare the transaction through slow-path.                       @*)
+    (*@     if gpp.phase == GPP_PREPARING {                                     @*)
+    (*@         _, prepared := gpp.srespm[rid]                                  @*)
+    (*@         if !prepared {                                                  @*)
+    (*@             return GPP_PREPARE                                          @*)
+    (*@         }                                                               @*)
+    (*@         return GPP_QUERY                                                @*)
+    (*@     }                                                                   @*)
+    (*@                                                                         @*)
+    wp_apply (wp_GroupPreparer__in _ GPPPreparing with "Hgpp").
+    iIntros (preparing) "Hgpp".
+    destruct preparing; wp_pures.
+    { iNamed "Hgpp". iNamed "Hsrespm".
+      wp_loadField.
+      wp_apply (wp_MapGet with "Hsrespm").
+      iIntros (b prepared) "[_ Hsrespm]".
+      wp_pures.
+      destruct prepared; wp_pures; last first.
+      { iApply ("HΦ" $! GPPPrepare).
+        iDestruct "Hsafe" as "[Hqv Hppsl]".
+        iFrame "Hfrespm Hvdm ∗ # %".
+        by iFrame "∗ #".
+      }
+      iApply ("HΦ" $! GPPQuery).
+      iFrame "Hfrespm Hvdm ∗ # %".
+      by iFrame "∗ #".
+    }
+
+    (*@     // Unprepare the transaction through slow-path.                     @*)
+    (*@     if gpp.phase == GPP_UNPREPARING {                                   @*)
+    (*@         _, unprepared := gpp.srespm[rid]                                @*)
+    (*@         if !unprepared {                                                @*)
+    (*@             return GPP_UNPREPARE                                        @*)
+    (*@         }                                                               @*)
+    (*@         return GPP_QUERY                                                @*)
+    (*@     }                                                                   @*)
+    (*@                                                                         @*)
+    wp_apply (wp_GroupPreparer__in _ GPPUnpreparing with "Hgpp").
+    iIntros (unpreparing) "Hgpp".
+    destruct unpreparing; wp_pures.
+    { iNamed "Hgpp". iNamed "Hsrespm".
+      wp_loadField.
+      wp_apply (wp_MapGet with "Hsrespm").
+      iIntros (b prepared) "[_ Hsrespm]".
+      wp_pures.
+      destruct prepared; wp_pures; last first.
+      { iApply ("HΦ" $! GPPUnprepare).
+        iFrame "Hfrespm Hvdm ∗ # %".
+        by iFrame "∗ #".
+      }
+      iApply ("HΦ" $! GPPQuery).
+      iFrame "Hfrespm Hvdm ∗ # %".
+      by iFrame "∗ #".
+    }
+
+    (*@     // Backup coordinator exists, just wait for the result.             @*)
+    (*@     if gpp.phase == GPP_WAITING {                                       @*)
+    (*@         return GPP_QUERY                                                @*)
+    (*@     }                                                                   @*)
+    (*@                                                                         @*)
+    wp_apply (wp_GroupPreparer__in _ GPPWaiting with "Hgpp").
+    iIntros (waiting) "Hgpp".
+    destruct waiting; wp_pures.
+    { iApply ("HΦ" $! GPPQuery). by iFrame. }
+
+    (*@     // The transaction has either prepared, committed, or aborted.      @*)
+    (*@     return GPP_REFRESH                                                  @*)
+    (*@ }                                                                       @*)
+    iApply ("HΦ" $! GPPRefresh). by iFrame.
+  Qed.
+
+End program.
