src/program_proof/tulip/program/quorum.v
@@ -1,6 +1,8 @@
 From Perennial.program_proof.tulip Require Import prelude.
 From Goose.github_com.mit_pdos.tulip Require Import quorum.
 
+(* Local Ltac Zify.zify_post_hook ::= Z.div_mod_to_equations. *)
+
 Section cquorum.
   Context `{!heapGS Σ}.
 
@@ -14,6 +16,39 @@ Section cquorum.
     (*@     return n / 2 + 1                                                    @*)
     (*@ }                                                                       @*)
     iIntros (Φ) "_ HΦ".
+    wp_rec. wp_pures.
+    iApply "HΦ".
+    iPureIntro. word.
+  Qed.
+
+  (* The precondition enforces no overflow. *)
+  Theorem wp_FastQuorum (n : u64) :
+    uint.Z n < 2 ^ 62 ->
+    {{{ True }}}
+      FastQuorum #n
+    {{{ (x : u64), RET #x; ⌜uint.Z x = ((3 * uint.Z n + 3) / 4)%Z⌝ }}}.
+  Proof.
+    (*@ func FastQuorum(n uint64) uint64 {                                      @*)
+    (*@     // ceiling(3n / 4)                                                  @*)
+    (*@     return (3 * n + 3) / 4                                              @*)
+    (*@ }                                                                       @*)
+    iIntros (Hn Φ) "_ HΦ".
+    wp_rec. wp_pures.
+    iApply "HΦ".
+    iPureIntro. word.
+  Qed.
+
+  Theorem wp_Half (n : u64) :
+    uint.Z n < 2 ^ 64 - 1 ->
+    {{{ True }}}
+      Half #n
+    {{{ (x : u64), RET #x; ⌜uint.Z x = ((uint.Z n + 1) / 2)%Z⌝ }}}.
+  Proof.
+    (*@ func Half(n uint64) uint64 {                                            @*)
+    (*@     // ceiling(n / 2)                                                   @*)
+    (*@     return (n + 1) / 2                                                  @*)
+    (*@ }                                                                       @*)
+    iIntros (Hn Φ) "_ HΦ".
     wp_rec. wp_pures.
     iApply "HΦ".
     iPureIntro. word.
